more array benchmarks translated

sv_manual_trans/array-examples/standard_copy5_true-unreach-call_ground.bpl
@@ -6,7 +6,6 @@ procedure main() returns (__RET: int)
   var a4: [int]int;
   var a5: [int]int;
   var a6: [int]int;
-  var a7: [int]int;
   var i: int;
   var x: int;
   i := 0;
@@ -54,24 +53,12 @@ procedure main() returns (__RET: int)
     a6[i] := a5[i];
     i := i + 1;
   }
-  i := 0;
-  while ((i<100000))
-  invariant (forall k : int :: (0 <= k && k < 100000) ==> a1[k] == a2[k]);
-  invariant (forall k : int :: (0 <= k && k < 100000) ==> a2[k] == a3[k]);
-  invariant (forall k : int :: (0 <= k && k < 100000) ==> a3[k] == a4[k]);
-  invariant (forall k : int :: (0 <= k && k < 100000) ==> a5[k] == a4[k]);
-  invariant (forall k : int :: (0 <= k && k < 100000) ==> a5[k] == a6[k]);
-  invariant (forall k : int :: (0 <= k && k < i) ==> a7[k] == a6[k]) && i <= 100000;
-  {
-    a7[i] := a6[i];
-    i := i + 1;
-  }
 
   x := 0;
   while ((x<100000))
-  invariant (forall k : int :: (0 <= k && k < 100000) ==> a1[k] == a7[k]);
+  invariant (forall k : int :: (0 <= k && k < 100000) ==> a1[k] == a6[k]);
   {
-    assert((a1[x]==a7[x]));
+    assert((a1[x]==a6[x]));
     x := x + 1;
   }
   __RET:=0;
