sv_manual_trans/array-examples/standard_compare_true-unreach-call_ground.bpl
@@ -1,0 +1,36 @@
+procedure main() returns (__RET: int)
+{
+  var a: [int]int;
+  var b: [int]int;
+  var i: int;
+  var rv: bool;
+  var x: int;
+  
+  i := 0;
+  rv := true;
+  while ((i<100000))
+  invariant rv ==> (forall k : int :: (0 <= k && k < i) ==> a[k] == b[k]);
+  {
+    if ((a[i]!=b[i]))
+    {
+      rv := false;
+    }
+
+    i := (i+1);
+  }
+
+  if (rv)
+  {
+    x := 0;
+    while ((x<100000))
+    invariant rv ==> (forall k : int :: (0 <= k && k < 100000) ==> a[k] == b[k]);
+    {
+      assert((a[x]==b[x]));
+      x := x + 1;
+    }  
+  }
+
+  __RET:=0;
+  return;
+}
+
