sv_manual_trans/array-examples/standard_copy3_true-unreach-call_ground.bpl
@@ -1,0 +1,42 @@
+procedure main() returns (__RET: int)
+{
+  var a1: [int]int;
+  var a2: [int]int;
+  var a3: [int]int;
+  var a4: [int]int;
+  var i: int;
+  var x: int;
+  i := 0;
+  while ((i<100000))
+  invariant (forall k : int :: (0 <= k && k < i) ==> a2[k] == a1[k]) && i <= 100000;
+  {
+    a2[i] := a1[i];
+    i := i + 1;
+  }
+  i := 0;
+  while ((i<100000))
+  invariant (forall k : int :: (0 <= k && k < 100000) ==> a1[k] == a2[k]);
+  invariant (forall k : int :: (0 <= k && k < i) ==> a2[k] == a3[k]) && i <= 100000;
+  {
+    a3[i] := a2[i];
+    i := i + 1;
+  }
+  i := 0;
+  while ((i<100000))
+  invariant (forall k : int :: (0 <= k && k < 100000) ==> a1[k] == a2[k]);
+  invariant (forall k : int :: (0 <= k && k < 100000) ==> a2[k] == a3[k]);
+  invariant (forall k : int :: (0 <= k && k < i) ==> a3[k] == a4[k]) && i <= 100000;
+  {
+    a4[i] := a3[i];
+    i := i + 1;
+  }
+  x := 0;
+  while ((x<100000))
+  invariant (forall k : int :: (0 <= k && k < 100000) ==> a1[k] == a4[k]);
+  {
+    assert((a1[x]==a4[x]));
+    x := x + 1;
+  }
+  __RET:=0;
+  return;
+}
